Examples: Rephrase assignment examples

src/panRefinementExampleScript.sml
@@ -1,9 +1,14 @@
 Theory panRefinementExample
-Ancestors panReducedSem panRefinement panPredicate
-Libs panRefinementLib
+Ancestors panReducedLang panReducedSem panPredicate panWeakestPrecondition panRefinement
+          finite_map[qualified] wordLang[qualified]
+Libs panRefinementLib BasicProvers[qualified] blastLib[qualified] HolSmtLib[qualified]
 
-Definition var_eq_def[simp]:
-  var_eq x (w : word64) = λs. FLOOKUP s.locals x = SOME (ValWord w)
+val refine_blast_tac = pan_refinement_tac_z3o;
+val refine_blast_thms_tac = pan_refinement_thms_tac_z3o;
+val blast_tac = HolSmtLib.Z3_ORACLE_TAC;
+
+Definition w64_def[simp]:
+  w64 (w : word64) = ValWord w
 End
 
 Definition fixed_def[simp]:
@@ -15,45 +20,108 @@ Definition postcond_def[simp]:
            (qt : 'a state -> bool) = λ(r,t). qr r ∧ qt t
 End
 
-Definition var_word[simp]:
+Definition var_word_def[simp]:
   var_word x = λs. case FLOOKUP s.locals x of
                    | SOME (ValWord w) => w
                    | _                => 0w
 End
 
 Theorem assignment_1:
-  Abbrev (P = var_eq x 0w) ∧
-  Abbrev (Q = postcond (fixed NONE) (var_eq x 10w)) ⇒
-  refine (HoareC P Q) (PanC (Assign Local x (Const 10w)))
+   refine
+     (HoareC (var_eq_val Local x (w64 0w))
+        (postcond (fixed NONE) (var_eq_val Local x (w64 10w))))
+     (PanC (Assign Local x (Const 10w)))
 Proof
   pan_refinement_tac assign_refinement_rule
 QED
 
-Theorem assignment_2_step_1:
-  Abbrev (P = var_eq x 0w) ∧
-  Abbrev (Q = postcond (fixed NONE) (var_eq x 10w)) ∧
-  Abbrev (QB = (λs. F)) ∧
-  Abbrev (QR = (λ(s,r). F)) ∧
-  Abbrev (QE = (λ(s,eid,e). F)) ∧
-  Abbrev (e = (Cmp Less (Var Local x) (Const 10w))) ∧
-  Abbrev (v = (λs. w2n (11w - var_word x s))) ∧
-  Abbrev (i = (λs. ∃w. var_eq x w s ∧ 0w ≤ w ∧ w ≤ 10w)) ⇒
-  refine (HoareC P Q)
-         (WhileC e i v (HoareC (while_body_pre i e) (while_body_post i QB QR QE)))
+Theorem assignment_2:
+   refine
+     (HoareC (var_eq_val Local x (w64 0w))
+        (postcond (fixed NONE) (var_eq_val Local x (w64 10w))))
+     (PanC
+        (While (Cmp Less (Var Local x) (Const 10w))
+           (Assign Local x (Op Add [Var Local x; Const 1w]))))
 Proof
-  pan_refinement_tac while_refinement_rule
+  rw[]
+  >> reverse (qsuff_tac ‘refine
+     (HoareC (var_eq_val Local x (w64 0w))
+        (postcond (fixed NONE) (var_eq_val Local x (w64 10w))))
+     (WhileC (Cmp Less (Var Local x) (Const 10w))
+        (λs. ∃w. var_eq_val Local x (w64 w) s ∧ 0w ≤ w ∧ w ≤ 10w)
+        (λs. w2n (-1w * var_word x s + 11w))
+        (HoareC
+           (while_body_pre
+              (λs. ∃w. var_eq_val Local x (w64 w) s ∧ 0w ≤ w ∧ w ≤ 10w)
+              (Cmp Less (Var Local x) (Const 10w)))
+           (while_body_post
+              (λs. ∃w. var_eq_val Local x (w64 w) s ∧ 0w ≤ w ∧ w ≤ 10w)
+              (λs. F) (λ(s,r). F) (λ(s,eid,e). F))))’)
+  >- (rpt (qpat_x_assum ‘refine _ _’ $ kall_tac)
+      >> qpat_abbrev_tac ‘P = (var_eq_val Local x (w64 0w))’
+      >> qpat_abbrev_tac ‘Q = (postcond (fixed NONE) (var_eq_val Local x (w64 10w)))’
+      >> qpat_abbrev_tac ‘e = (Cmp Less (Var Local x) (Const 10w))’
+      >> qpat_abbrev_tac ‘i = (λs. ∃w. var_eq_val Local x (w64 w) s ∧ 0w ≤ w ∧ w ≤ 10w)’
+      >> qpat_abbrev_tac ‘v = (λs. w2n (-1w * var_word x s + 11w))’
+      >> qpat_abbrev_tac ‘QB = (λs. F)’
+      >> qpat_abbrev_tac ‘QR = (λ(s,r). F)’
+      >> qpat_abbrev_tac ‘QE = (λ(s,eid,e). F)’
+      >> refine_blast_tac while_refinement_rule)
+  >> rw[]
+  >> reverse (qsuff_tac ‘refine
+     (WhileC (Cmp Less (Var Local x) (Const 10w))
+        (λs. ∃w. var_eq_val Local x (w64 w) s ∧ 0w ≤ w ∧ w ≤ 10w)
+        (λs. w2n (-1w * var_word x s + 11w))
+        (HoareC
+           (while_body_pre
+              (λs. ∃w. var_eq_val Local x (w64 w) s ∧ 0w ≤ w ∧ w ≤ 10w)
+              (Cmp Less (Var Local x) (Const 10w)))
+           (while_body_post
+              (λs. ∃w. var_eq_val Local x (w64 w) s ∧ 0w ≤ w ∧ w ≤ 10w)
+              (λs. F) (λ(s,r). F) (λ(s,eid,e). F))))
+     (WhileC (Cmp Less (Var Local x) (Const 10w))
+        (λs. ∃w. var_eq_val Local x (w64 w) s ∧ 0w ≤ w ∧ w ≤ 10w)
+        (λs. w2n (-1w * var_word x s + 11w))
+        (PanC (Assign Local x (Op Add [Var Local x; Const 1w]))))’)
+  >- (reverse (qsuff_tac ‘refine
+     (HoareC
+        (while_body_pre
+           (λs. ∃w. var_eq_val Local x (w64 w) s ∧ 0w ≤ w ∧ w ≤ 10w)
+           (Cmp Less (Var Local x) (Const 10w)))
+        (while_body_post
+           (λs. ∃w. var_eq_val Local x (w64 w) s ∧ 0w ≤ w ∧ w ≤ 10w) (λs. F)
+           (λ(s,r). F) (λ(s,eid,e). F)))
+     (PanC (Assign Local x (Op Add [Var Local x; Const 1w])))’)
+      >- (rpt (qpat_x_assum ‘refine _ _’ $ kall_tac)
+          >> qpat_abbrev_tac ‘e = (Cmp Less (Var Local x) (Const 10w))’
+          >> qpat_abbrev_tac ‘i = (λs. ∃w. var_eq_val Local x (w64 w) s ∧ 0w ≤ w ∧ w ≤ 10w)’
+          >> qpat_abbrev_tac ‘QB = (λs. F)’
+          >> qpat_abbrev_tac ‘QR = (λ(s,r). F)’
+          >> qpat_abbrev_tac ‘QE = (λ(s,eid,e). F)’
+          >> gvs[]
+          >> refine_blast_tac assign_refinement_rule)
+      >> rw[]
+      >> gvs[refine_monotonic_while])
+  >> rw[]
+  >> drule_all_then assume_tac refine_transitive
+  >> reverse (qsuff_tac ‘refine
+     (WhileC (Cmp Less (Var Local x) (Const 10w))
+        (λs. ∃w. var_eq_val Local x (w64 w) s ∧ 0w ≤ w ∧ w ≤ 10w)
+        (λs. w2n (-1w * var_word x s + 11w))
+        (PanC (Assign Local x (Op Add [Var Local x; Const 1w]))))
+     (PanC
+        (While (Cmp Less (Var Local x) (Const 10w))
+           (Assign Local x (Op Add [Var Local x; Const 1w]))))’)
+  >- (rpt (qpat_x_assum ‘refine _ _’ $ kall_tac)
+      >> qpat_abbrev_tac ‘e = (Cmp Less (Var Local x) (Const 10w))’
+      >> qpat_abbrev_tac ‘i = (λs. ∃w. var_eq_val Local x (w64 w) s ∧ 0w ≤ w ∧ w ≤ 10w)’
+      >> qpat_abbrev_tac ‘v = (λs. w2n (-1w * var_word x s + 11w))’
+      >> refine_blast_thms_tac while_refinement_rule_pan [evaluate_def])
+  >> rw[]
+  >> drule_all_then assume_tac refine_transitive
+  >> gvs[]
 QED
 
-Theorem assignment_2_step_2:
-  Abbrev (P  = (while_body_pre i e)) ∧
-  Abbrev (Q  = (while_body_post i QB QR QE)) ∧
-  Abbrev (QB = (λs. F)) ∧
-  Abbrev (QR = (λ(s,r). F)) ∧
-  Abbrev (QE = (λ(s,eid,e). F)) ∧
-  Abbrev (e  = (Cmp Less (Var Local x) (Const 10w))) ∧
-  Abbrev (i = (λs. ∃w. var_eq x w s ∧ 0w ≤ w ∧ w ≤ 10w)) ⇒
-  refine (HoareC P Q)
-         (PanC (Assign Local x (Op Add [(Var Local x); (Const 1w)])))
 Proof
   pan_refinement_tac assign_refinement_rule
 QED
